src/pp.lean
@@ -1,0 +1,213 @@
+import init.data.list
+import init.data.to_string
+
+import data.bitvec
+import data.rbmap
+
+import .ast
+
+import tactic.linarith
+
+namespace sized
+
+def map {a b:Type} [has_sizeof a] (sz:ℕ) (f : Πx:a, sizeof x < sz → b) : Πxs:list a, (sizeof xs <= sz) → list b
+| [] _      := []
+| (x::xs) H :=
+   have Hx  : sizeof x  <  sz, by { unfold sizeof has_sizeof.sizeof list.sizeof at *, linarith },
+   have Hxs : sizeof xs <= sz, by { unfold sizeof has_sizeof.sizeof list.sizeof at *, linarith },
+   f x Hx :: map xs Hxs
+.
+
+@[reducible]
+def map_over {a b:Type} [has_sizeof a] (xs:list a) (f : Πx:a, sizeof x < sizeof xs → b) : list b :=
+  map (sizeof xs) f xs (nat.less_than_or_equal.refl _).
+
+end sized
+
+namespace pp
+
+reserve infixl ` <> `: 50
+reserve infixl ` <+> `: 50
+reserve infixl ` <$> `: 60
+
+structure doc : Type := (compose : string → string).
+
+def text (x:string) := doc.mk (λz, x ++ z).
+def render (x:doc) : string := x.compose "".
+def to_doc {a:Type} [has_to_string a] : a → doc := text ∘ to_string.
+
+def empty : doc := doc.mk (λ z, z).
+def next_to (x y : doc) : doc := doc.mk (x.compose ∘ y.compose).
+infix <>  := next_to.
+
+def spacesep (x y:doc) : doc  := x <> text " " <> y
+def linesep (x y:doc)  : doc  := x <> text "\n" <> y.
+
+infix <+> := spacesep.
+infix <$> := linesep.
+
+def hcat (xs:list doc) : doc := list.foldr next_to empty xs.
+def vcat (xs:list doc) : doc := list.foldr linesep empty xs.
+
+def punctuate (p:doc) : list doc → list doc
+| [ ]     := []
+| (x::xs) := x :: (list.foldr (λ a b, p :: a :: b) [] xs)
+.
+
+def nat : ℕ → doc := text ∘ to_string
+def int : ℤ → doc := text ∘ to_string
+
+def pp_nonzero : ℕ → doc
+| nat.zero := empty
+| n := nat n
+.
+
+def surrounding (first last : string) (x:doc) : doc :=
+  text first <> x <> text last
+
+def parens   : doc → doc := surrounding "(" ")"
+def brackets : doc → doc := surrounding "[" "]"
+def angles   : doc → doc := surrounding "<" ">"
+def braces   : doc → doc := surrounding "{" "}"
+
+def comma : doc := text ","
+def commas : list doc → doc := hcat ∘ punctuate comma
+
+end pp
+
+
+namespace llvm
+open pp
+
+section layout_spec.
+open layout_spec.
+
+def pp_layout_body (sz abi:ℕ) (pref: option ℕ) : doc :=
+  nat sz <> text ":" <> nat abi <>
+    (option.rec empty (λx, text ":" <> nat x) pref)
+.
+
+def pp_align_type : align_type → doc
+| align_type.integer := text "i"
+| align_type.vector  := text "v"
+| align_type.float   := text "f"
+| align_type.aggregate := text "a"
+.
+
+def pp_mangling : mangling → doc
+| mangling.elf := text "e"
+| mangling.mips := text "m"
+| mangling.mach_o := text "o"
+| mangling.windows_coff     := text "w"
+| mangling.windows_coff_x86 := text "x"
+.
+
+def pp_layout_spec : layout_spec → doc
+| big_endian     := text "E"
+| little_endian  := text "e"
+| (pointer_size addr_space sz abi pref _idx) :=
+     text "p" <> pp_nonzero addr_space <> text ":" <> pp_layout_body sz abi pref
+| (align_size tp sz abi pref) :=
+     pp_align_type tp <> pp_layout_body sz abi pref
+| (native_int_size szs) := text "n" <> hcat (punctuate (text ":") (list.map nat szs))
+| (stack_align n) := text "S" <> nat n
+| (layout_spec.mangling m)     := text "m:" <> pp_mangling m
+| (function_address_space n)  := text "P" <> nat n
+| (stack_alloca n) := text "A" <> nat n
+.
+
+def pp_layout (xs:data_layout) : doc
+  := hcat (punctuate (text "-") (list.map pp_layout_spec xs))
+.
+
+def l1 : data_layout :=
+  [ big_endian,
+    layout_spec.mangling mangling.mach_o,
+    pointer_size 0 64 64 none 0,
+    align_size align_type.integer 64 64 none,
+    align_size align_type.float   80 128 none,
+    align_size align_type.float   64 64 none,
+    native_int_size [8,16,32,64],
+    stack_align 128
+  ]
+
+end layout_spec.
+
+
+def pp_ident (n:ident) : doc :=
+  text "%" <> text (n.ident)  -- FIXME! deal with the 'validIdentifier' question
+.
+
+def pp_symbol (n:symbol) : doc :=
+  text "@" <> text (n.symbol)
+.
+
+def pp_label : block_label → doc
+| (block_label.named i) := pp_ident i
+| (block_label.anon n)  := text "%" <> to_doc n
+.
+
+def packed_braces : doc → doc := surrounding "<{" "}>"
+
+def pp_type : llvm_type → doc := λ_, empty.
+
+
+meta def pp_tac :=
+  `[unfold has_well_founded_of_has_sizeof has_well_founded.r sizeof_measure measure
+      inv_image sizeof has_sizeof.sizeof psum.sizeof typed.sizeof const_expr.sizeof value.sizeof
+      at *,
+      repeat { rw llvm.typed.sizeof_spec' at *, unfold sizeof has_sizeof.sizeof at * },
+      try { linarith }
+   ].
+
+def pp_conv_op : conv_op → doc
+| conv_op.trunc      := text "trunc"
+| conv_op.zext       := text "zext"
+| conv_op.sext       := text "sext"
+| conv_op.fp_trunc   := text "fptrunc"
+| conv_op.fp_ext     := text "fpext"
+| conv_op.fp_to_ui   := text "fptoui"
+| conv_op.fp_to_si   := text "fptosi"
+| conv_op.ui_to_fp   := text "uitofp"
+| conv_op.si_to_fp   := text "sitofp"
+| conv_op.ptr_to_int := text "ptrtoint"
+| conv_op.int_to_ptr := text "inttoptr"
+| conv_op.bit_cast   := text "bitcast"
+.
+
+mutual def pp_value, pp_const_expr
+with pp_value : value → doc
+| value.null           := text "null"
+| value.undef          := text "undef"
+| value.zero_init      := text "0"
+| (value.integer i)    := to_doc i
+| (value.bool b)       := to_doc b
+| (value.ident n)      := pp_ident n
+| (value.symbol n)     := pp_symbol n
+| (value.const_expr e) := pp_const_expr e
+| (value.label l)      := pp_label l
+| (value.array tp vs)  := brackets (commas (sized.map_over vs (λv H, pp_type tp <+> pp_value v)))
+| (value.vector tp vs) := angles (commas (sized.map_over vs (λv H, pp_type tp <+> pp_value v)))
+| (value.struct fs)    := braces (commas (sized.map_over fs (λf H, pp_type (f.type) <+> pp_value (f.value))))
+| (value.packed_struct fs) := packed_braces (commas (sized.map_over fs (λf H, pp_type (f.type) <+> pp_value (f.value))))
+
+with pp_const_expr : const_expr → doc
+| (const_expr.select cond x y) :=
+     text "select" <+>
+     pp_type (typed.type cond) <+> pp_value (typed.value cond) <+>
+     text "," <+>
+     pp_type (typed.type x) <+> pp_value (typed.value x) <+> text "," <+>
+     pp_value (typed.value y)
+| (const_expr.gep inbounds inrange tp vs) :=
+    text "getelementpointer" <+>
+    (if inbounds then text "inbounds " else empty) <>
+    parens ( pp_type tp <> comma <+> commas (sized.map_over vs (λ v H, pp_type (typed.type v) <+> pp_value (typed.value v))))
+
+| (const_expr.conv op x tp) :=
+    pp_conv_op op <+> parens (pp_type (typed.type x) <+> pp_value (typed.value x) <+> text "to" <+> pp_type tp)
+
+using_well_founded ⟨λ _ _, `[exact (has_well_founded_of_has_sizeof _)] , pp_tac⟩
+.
+
+
+end llvm.
